no need for a retract

main.v
@@ -13,6 +13,8 @@ Unset Printing Implicit Defensive.
 Reserved Notation "x [ s ]" (at level 30).
 (* substitution in the syntax *)
 Reserved Notation "x [ s ]ₛ" (at level 30).
+(* substitution in the quotiented syntax *)
+Reserved Notation "x [ s ]ₘ" (at level 30).
 (* mixed substitution in the syntax *)
 Reserved Notation "x ⟦ s ⟧" (at level 30).
 
@@ -75,6 +77,19 @@ Definition vec_map_fun_ext {A B C : Type}(f g : A -> B -> C) {l : list A}
   induction v; cbn; congruence.
 Defined.
 
+Lemma vec_map_map_swap {A B B' C C' D : Type}
+      (f  : A -> B -> C ) (g  : A -> C -> D)
+      (f' : A -> B -> C') (g' : A -> C' -> D)
+      (fg_f'g' : forall a b, g a (f a b) = g' a (f' a b))
+      {l : list A}
+      (v : Vec B l) : Vec_map g (Vec_map f v) =
+                       Vec_map g' (Vec_map f' v) .
+Proof.
+  rewrite 2 vec_map_map.
+  apply vec_map_fun_ext.
+  assumption.
+Qed.
+
 
 (* shifts on renamings *)
 Definition shiftₙ (n : nat) (f : nat -> nat)  : nat -> nat :=
@@ -93,6 +108,10 @@ Lemma commutes_if {A B : Type}(f : A -> B)(b : bool) x y :
   (if b then f x else f y) = f (if b then x else y).
 Proof.
 destruct b; reflexivity.
+Qed.
+Lemma if_if {A : Type}(b : bool) (x y z : A) :
+  (if b then if b then x else y else z) = (if b then x else z).
+  destruct b ; reflexivity.
 Qed.
 
 Lemma shiftₙₛ_natural
@@ -251,7 +270,7 @@ Proof.
     eapply shiftₙₛ_ext.
     + reflexivity.
     + apply eq.
-Qed.
+Defined.
 
 Fixpoint Z_ren_subst_eq {S} (f : nat -> nat) (x : Z S) :
   Z_ren f x = x [ fun n => Var S (f n) ]ₛ.
@@ -325,6 +344,183 @@ Proof.
     + reflexivity.
 Qed.
 
+Require Import micromega.Lia.
+Lemma shiftₙₛ_shiftₙ {X : Type}(var : nat -> X)(ren : (nat -> nat) -> (X -> X))(n m : nat) (f : nat -> X)g :
+  shiftₙₛ var ren n f (shiftₙ n g m) = shiftₙₛ var ren n (fun n0 : nat => f (g n0)) m.
+Proof.
+  unfold shiftₙₛ, shiftₙ.
+  cbn -[leb].
+  destruct (m <? n) eqn:e.
+  - rewrite e.
+    reflexivity.
+  - case(Nat.ltb_spec _ _).
+    + intro. exfalso. lia.
+    + intros.
+      rewrite Nat.add_sub.
+      reflexivity.
+Qed.
+
+(*
+Lemma shiftₙ_shiftₙ g f a n : 
+  (shiftₙ a g ∘ shiftₙ a f) n = shiftₙ a (g ∘ f) n.
+Proof.
+  unfold compose.
+  cbn.
+  unfold shiftₙₛ, shiftₙ.
+  destruct (n <? a) eqn:e.
+  - rewrite e.
+    reflexivity.
+  - case(Nat.ltb_spec _ _).
+    + intro. exfalso. lia.
+    + intros. f_equal.
+      f_equal.
+      lia.
+Qed.
+*)
+Fixpoint Z_ren_subst {S : signature} g f (z : Z S) :
+Z_ren g z [ f ]ₛ = z [ fun n => f (g n)  ]ₛ.
+Proof.
+  destruct z.
+  - reflexivity.
+  - cbn.
+    f_equal.
+    rewrite vec_map_map.
+    apply vec_map_fun_ext.
+    intros.
+    cbn.
+    etransitivity;[apply Z_ren_subst|].
+    apply Z_subst_ext.
+    intro n.
+    apply shiftₙₛ_shiftₙ.
+Qed.
+
+Lemma Z_ren_ren {S : signature} g f (z : Z S) :
+Z_ren g (Z_ren f z) = Z_ren (g ∘ f) z.
+  rewrite Z_ren_subst_eq at 1.
+  rewrite Z_ren_subst.
+  symmetry.
+  apply Z_ren_subst_eq.
+Qed.
+
+
+  (* Z_ren (shiftₙ a g) (shiftₙₛ (Var S) Z_ren a f n) = shiftₙₛ (Var S) Z_ren a (fun n0 : nat => Z_ren g (f n0)) n *)
+(* TODO: factoriser un principe de recurrence *)
+Fixpoint Z_subst_ren {S : signature} g f (z : Z S) :
+Z_ren g (z [ f ]ₛ) = z [ fun n => Z_ren g (f n)  ]ₛ.
+Proof.
+  destruct z.
+  - reflexivity.
+  - cbn.
+    f_equal.
+    rewrite vec_map_map.
+    apply vec_map_fun_ext.
+    intros.
+    cbn.
+    etransitivity;[apply Z_subst_ren|].
+    apply Z_subst_ext.
+    intro n.
+
+  unfold shiftₙ, shiftₙₛ.
+  cbn -[leb].
+  rewrite <- (commutes_if (Z_ren _)).
+  cbn -[leb].
+  destruct (n <? a) eqn:eqna.
+  + reflexivity.
+  + cbn -[leb].
+    rewrite Z_ren_ren.
+    rewrite Z_ren_ren.
+    rewrite 2 Z_ren_subst_eq.
+    apply Z_subst_ext.
+    intro m.
+    unfold compose.
+    cbn -[leb].
+    case(Nat.ltb_spec _ _).
+    * intro. exfalso. lia.
+    * intros. 
+      rewrite Nat.add_sub.
+      reflexivity.
+Qed.
+
+Fixpoint Z_subst_subst {S : signature}
+      (f g : nat -> Z S) (x : Z S) :
+  (x [g]ₛ) [f]ₛ = x [fun n : nat => g n [f]ₛ]ₛ.
+Proof.
+  destruct x.
+  - reflexivity.
+  - cbn.
+    f_equal.
+    rewrite vec_map_map.
+    apply vec_map_fun_ext.
+    intros.
+    cbn.
+    etransitivity;[apply Z_subst_subst|].
+    apply Z_subst_ext.
+    intro n.
+    cbn.
+    (* ca devrait marcher *)
+  unfold shiftₙ, shiftₙₛ.
+  cbn -[leb].
+  rewrite <- (commutes_if (Z_subst _)).
+  cbn -[leb].
+  rewrite if_if.
+  destruct (n <? a) eqn:eqna.
+  + reflexivity.
+  + cbn -[leb].
+    rewrite Z_ren_subst.
+    erewrite Z_subst_ext; revgoals.
+    {
+      intro.
+  - case(Nat.ltb_spec _ _).
+    + intro. exfalso. lia.
+    + intros. f_equal.
+      rewrite Nat.add_sub.
+      reflexivity.
+      }
+    symmetry.
+    apply Z_subst_ren.
+    Qed.
+
+Fixpoint Vec_map_id {A B : Type}{l : list A}(v : Vec B l) : Vec_map (fun _ x => x) v = v.
+  destruct v.
+  -  reflexivity.
+  -  cbn.
+     f_equal.
+     apply Vec_map_id.
+Defined.
+
+Lemma shiftₙ_id (n : nat) (p : nat)  : 
+  shiftₙ n (fun x => x) p = p.
+  unfold shiftₙ.
+  case (Nat.ltb_spec).
+  + reflexivity.
+  + lia.
+Qed.
+
+Lemma shiftₙₛ_var {X : Type}(var : nat -> X)ren
+      (eq_ren : forall f n, ren f (var n) = var (f n))
+      n m : shiftₙₛ var ren n var m = var m.
+Proof.
+    unshelve erewrite <- (var_shiftₙ _ _ (fun n => n)).
+    + auto.
+    + cbn.
+      f_equal.
+      apply shiftₙ_id.
+Qed.
+Fixpoint Z_subst_id {S} (z : Z S) : z [Var S ]ₛ = z.
+  destruct z.
+  - reflexivity.
+  - cbn.
+    f_equal.
+    etransitivity;[|apply Vec_map_id].
+    apply vec_map_fun_ext.
+    intros.
+    etransitivity;[|apply Z_subst_id].
+    apply Z_subst_ext.
+    intro n.
+    apply shiftₙₛ_var.
+    reflexivity.
+Qed.
+  
 
 Lemma Z_model_laws (S : signature) : model_laws (Z_model_data S).
 Proof.
@@ -340,10 +536,10 @@ Proof.
     unfold shiftₙₛ.
     rewrite Z_ren_subst_eq.
     reflexivity.
-  - admit.
-  - admit.
+  - apply Z_subst_subst. 
+  - apply Z_subst_id.
+Qed.
 
-Admitted.
 
 Definition ZModel (S : signature) : model S :=
   {| data := Z_model_data S; laws := Z_model_laws S |}.
@@ -487,6 +683,24 @@ Lemma rel_vec_rfl (rx : forall x, R x x) l (v : Vec B l) : rel_vec v v.
 Qed.
   End relvec.
 
+(* class_ind : forall [X : Type] [r : Eqv X] (P : X // r -> Prop), (forall x : X, P (x / r)) -> forall x : X // r, P x *)
+Fixpoint vec_quot_ind
+         {A B : Type}{R : Eqv B}{l : list A}
+         (P : Vec (B // R) l -> Prop)
+         (Pquot : forall (v : Vec B l), P (Vec_map (fun _ => class R) v)) 
+         (v : Vec (B // R) l) : P v.
+Proof.
+  destruct v as [|a l b v].
+  - apply (Pquot (NilV _)).
+  - cbn.
+    revert v b.
+    unshelve refine (vec_quot_ind _  _ _ _ _  _).
+    +  intros v b.
+       revert b v.
+       unshelve refine (class_ind _ _).
+       exact (fun b v => Pquot (ConsV a b v )).
+Qed.
+
 Fixpoint vec_quot_out (A B C : Type)(R : Eqv B)(l : list A)(f : Vec B l -> C)
       (compat_f : forall b b', rel_vec R b b' -> f b = f b')
       (v : Vec (B // R) l) : C.
@@ -531,6 +745,54 @@ Proof.
     rewrite vec_quot_out_proj.
     rewrite factorize.
     reflexivity.
+Qed.
+
+Fixpoint finitary_seq_quot_ind
+         {B : Type}{R : Eqv B}
+         (P : (nat -> (B // R)) -> Prop)
+         (n : nat)
+         (Pn : forall f g, (forall p, p < n -> f p = g p) -> P f -> P g)
+         (Pq : forall f, P (class R ∘ f)) f {struct n}: P f.
+Proof.
+  destruct n.
+  - generalize (f 0).
+    apply class_ind.
+    intro b.
+    eapply Pn.
+    + intros p hp.
+      exfalso.
+      inversion hp.
+    + unshelve apply Pq.
+      intro n.
+      exact b.
+  -
+    remember (f n) as b' eqn:eqb'.
+    cut (P (fun p => if p =? n then b' else f p)) .
+    + eapply Pn.
+      intro p.
+      case (Nat.eqb_spec); intros;congruence.
+    + clear eqb'.
+      revert b'.
+    refine (class_ind _ _).
+    intro b.
+    pattern f.
+    revert f.
+    eapply (finitary_seq_quot_ind B R _ n).
+    * intros f g  Pfg hf.
+      unshelve eapply (Pn _ _ _ hf).
+      cbn.
+      intros p hp.
+      case (Nat.eqb_spec).
+      -- reflexivity.
+      -- intro.
+         apply Pfg.
+         lia.
+    * intro f.
+      cut (P (fun p => class R (if p =? n then b else f p))).
+      -- eapply Pn.
+         intro.
+         case (Nat.eqb_spec); reflexivity.
+      -- apply Pq.
 Qed.
 
 
@@ -710,30 +972,84 @@ Proof.
       apply ZE_ren_proj.
 Qed.
 
+Fixpoint vec_max {A : Type}(l : list A) (v : Vec nat l) : nat :=
+  match v with
+    NilV _ => 0
+  | ConsV a b lB => Nat.max b (vec_max lB)
+    end.
 
-(*necessite l'axiome du choix (lift_fun) *)
+Fixpoint max_fv {S : signature} (z : Z S) : nat :=
+  match z with
+    Var _ n => n
+  | Op op  v => vec_max (Vec_map (fun n x => n + max_fv x) v)
+  end.
+
+Fixpoint ZE_mixed_subst_max_fv {E} (f g : nat -> ZE E)(z : Z _)
+         (hfg : forall n, n <= max_fv z -> f n = g n) {struct z} :
+  z ⟦ f ⟧ = z ⟦ g ⟧.
+Proof.
+  destruct z.
+  - cbn in hfg.
+    cbn.
+    apply hfg.
+    reflexivity.
+  - cbn.
+    f_equal.
+    cbn in hfg.
+    revert hfg.
+    induction v.
+    + reflexivity.
+    + cbn.
+      intro hfg.
+      f_equal.
+      * apply ZE_mixed_subst_max_fv.
+        intros.
+        unfold shiftₙₛ.
+        case (Nat.ltb_spec).
+        -- reflexivity.
+        -- intros.
+           f_equal.
+           cbn in hfg.
+           apply hfg.
+           lia.
+           (* apply h. *)
+           (* lia. *)
+      * apply IHv.
+        cbn.
+        intros.
+        apply hfg.
+        lia.
+Qed.
+
 Fixpoint ZE_mixed_subst_compat
   (E : equational_theory) 
       (f : nat -> ZE E)(z z' : Z (main_signature E))(rz :ZEr E z z'): z ⟦ f ⟧ = z' ⟦ f ⟧.
 Proof.
   destruct rz.
   - cbn.
-    destruct (lift_fun f) as [h heq].
-    rewrite heq.
-    do 2 rewrite <- (Z_subst_quot h).
-    etransitivity.
-    {
-    apply (f_equal projE).
-    apply  (lift_ops_subst _ (m := ZModel _) v h).
-    }
-    etransitivity;revgoals.
-    {
-      symmetry.
-    apply (f_equal projE).
-    apply  (lift_ops_subst _ (m := ZModel _) v h).
-    }
-    apply class_eq.
-    constructor.
+    revert f.
+    refine (finitary_seq_quot_ind (n := 1 + Nat.max (max_fv(left_handside E (ZModel (main_signature E)) o v))
+                                  (max_fv (right_handside E (ZModel (main_signature E)) o v))) _ _).
+    + intros f g hfg.
+      erewrite 2 (ZE_mixed_subst_max_fv (f := f)(g := g)).
+      * tauto.
+      * intros; apply hfg; lia.
+      * intros; apply hfg; lia.
+    + intro h.
+      do 2 rewrite <- (Z_subst_quot h).
+      etransitivity.
+      {
+        apply (f_equal projE).
+        apply  (lift_ops_subst _ (m := ZModel _) v h).
+      }
+      etransitivity;revgoals.
+      {
+        symmetry.
+        apply (f_equal projE).
+        apply  (lift_ops_subst _ (m := ZModel _) v h).
+      }
+      apply class_eq.
+      constructor.
   - reflexivity.
   - symmetry.
     apply ZE_mixed_subst_compat.
@@ -761,7 +1077,123 @@ Definition ZE_subst {E : equational_theory}  (f : nat -> ZE E) (x : ZE E) : ZE E
     apply ZE_mixed_subst_compat.
     assumption.
 Defined.
+
+Notation "x [ f ]ₘ" := (ZE_subst f x) (at level 30).
+
+Lemma ZE_subst_proj {E : equational_theory} f z  :
+  projE (E := E) z [ f ]ₘ = z ⟦ f ⟧.
+Proof.
+  unfold ZE_subst, projE.
+  rewrite factorize.
+  reflexivity.
+Qed.
+Lemma ZE_subst_proj_proj {E : equational_theory} f z  :
+  projE (E := E) z [ projE ∘ f ]ₘ = projE (z [ f ]ₛ).
+Proof.
+  etransitivity; [apply ZE_subst_proj|].
+  symmetry.
+  apply Z_subst_quot.
+Qed.
+
+Lemma ZE_subst_ext {E}(f g : nat -> ZE E) (fg : forall n : nat, f n = g n) : forall x : ZE E, x [ f ]ₘ = x [ g ]ₘ.
+Proof.
+  apply class_ind.
+  intro z.
+  rewrite  2 (ZE_subst_proj _ z).
+  apply ZE_mixed_subst_ext.
+  assumption.
+Qed.
+
+Lemma ZE_ren_var {E}(f : nat -> nat) (n : nat): ZE_ren (E := E) f (VarE n) = VarE (f n).
+Proof.
+  unfold ZE_ren, VarE.
+  rewrite factorize1.
+  reflexivity.
+Qed.
       
+Lemma ZE_subst_var {E} x f :
+  VarE (E := E) x [ f ]ₘ = f x.
+Proof.
+  unfold ZE_subst, VarE.
+  rewrite factorize.
+  reflexivity.
+Qed.
+Lemma shiftₛ_projE {E} n f x :
+  shiftₛ (VarE (E := E)) ZE_subst n (projE ∘ f) x =
+  projE (shiftₛ (Var _) Z_subst n f x).
+Proof.
+  symmetry.
+  apply (shiftₙₛ_natural (g:= projE)).
+  - reflexivity.
+  - intros g z.
+    symmetry.
+    apply ZE_subst_proj_proj.
+Qed.
+
+(* Lemma projE_subst_max_fv {E} *)
+(*       (f g : nat -> ZE E)(z : Z _) *)
+(*          (hfg : forall n, n <= max_fv z -> f n = g n) : *)
+(*   projE z [f ]ₘ = projE z [f ]ₘ *)
+Lemma ZE_ren_subst_eq {E} (f : nat -> nat) (x : ZE E) :
+  ZE_ren f x = x [ fun n => VarE (f n) ]ₘ.
+Proof.
+  revert x.
+  apply class_ind.
+  intro z.
+  fold (projE z).
+  symmetry.
+  etransitivity;[|apply  ZE_ren_proj].
+  etransitivity;[apply ZE_subst_proj_proj|].
+  f_equal.
+  symmetry.
+  apply Z_ren_subst_eq.
+Qed.
+
+Lemma ZE_ops_ren
+  {E : equational_theory} (o : O (main_signature E)) (v : Vec (ZE E) (ar o)) (f : nat -> nat) :
+    ZE_ren f (ZE_ops v) = ZE_ops (Vec_map (fun (n : nat) (t : ZE E) => ZE_ren (shiftₙ n f) t) v).
+Proof.
+  revert v.
+  refine (vec_quot_ind _).
+  intro v.
+  rewrite ZE_ops_projE.
+  rewrite <- ZE_ren_proj.
+  cbn.
+  rewrite <- ZE_ops_projE.
+  f_equal.
+  rewrite vec_map_map.
+  rewrite vec_map_map.
+
+  apply vec_map_fun_ext.
+  intros.
+  apply ZE_ren_proj.
+Qed.
+
+Lemma ZE_ops_subst
+  {E : equational_theory} (o : O (main_signature E)) (v : Vec (ZE E) (ar o)) (f : nat -> ZE E) :
+    ZE_ops v [f ]ₘ = ZE_ops (Vec_map (fun (n : nat) (t : ZE E) => t [shiftₛ VarE ZE_subst n f ]ₘ) v).
+Proof.
+  revert v.
+  refine (vec_quot_ind _).
+  intro v.
+  rewrite ZE_ops_projE.
+  rewrite ZE_subst_proj.
+  cbn.
+  f_equal.
+  rewrite vec_map_map.
+  apply vec_map_fun_ext.
+  intros.
+  symmetry.
+  etransitivity.
+  apply ZE_subst_proj.
+  apply ZE_mixed_subst_ext.
+  intro n.
+  apply shiftₙₛ_ext.
+  -  intros. symmetry. 
+     apply ZE_ren_subst_eq.
+  - reflexivity.
+Qed.
+
 Definition ZEModel_data (E : equational_theory) : model_data (main_signature E) :=
   {|
   carrier := ZE E;
@@ -770,10 +1202,196 @@ Definition ZEModel_data (E : equational_theory) : model_data (main_signature E) 
   substitution := ZE_subst
   |}.
 
+
+Fixpoint ZE_ren_mixed_subst {E} (g : nat -> nat) (f : nat -> ZE E) (z : Z _) :
+  Z_ren g z ⟦ f ⟧ = z ⟦ fun n : nat => f (g n) ⟧.
+Proof.
+  destruct z.
+  - reflexivity.
+  - cbn.
+    f_equal.
+    rewrite vec_map_map.
+    apply vec_map_fun_ext.
+    intros.
+    cbn.
+    etransitivity;[apply ZE_ren_mixed_subst|].
+    apply ZE_mixed_subst_ext.
+    intro n.
+    (* ca devrait marcher *)
+  unfold shiftₙ, shiftₙₛ.
+  cbn -[leb].
+  cbn -[leb].
+  destruct (n <? a) eqn:eqna.
+  + rewrite eqna; reflexivity.
+  + cbn -[leb].
+    case(Nat.ltb_spec _ _).
+    * intro. exfalso. lia.
+    * intros. f_equal.
+      rewrite Nat.add_sub.
+      reflexivity.
+Qed.
+
+Lemma ZE_ren_subst {E} (g : nat -> nat) (f : nat -> ZE E) (z : ZE E) :
+ZE_ren g z [f ]ₘ = z [fun n : nat => f (g n) ]ₘ.
+Proof.
+  revert z.
+  apply class_ind.
+  intro z.
+  fold (projE z).
+  rewrite <- ZE_ren_proj.
+  rewrite ZE_subst_proj.
+  rewrite ZE_subst_proj.
+  apply ZE_ren_mixed_subst.
+Qed.
+Lemma ZE_ren_ren {E} g f (z : ZE E) :
+ZE_ren g (ZE_ren f z) = ZE_ren (g ∘ f) z.
+  rewrite ZE_ren_subst_eq at 1.
+  rewrite ZE_ren_subst.
+  symmetry.
+  apply ZE_ren_subst_eq.
+Qed.
+Fixpoint ZE_mixed_subst_ren 
+  {E} (g : nat -> nat) (f : nat -> ZE E) z :
+  ZE_ren g (z ⟦ f ⟧) = z ⟦ fun n : nat => ZE_ren g (f n) ⟧.
+Proof.
+  destruct z.
+  - reflexivity.
+  - cbn.
+    rewrite ZE_ops_ren.
+    f_equal.
+    rewrite vec_map_map.
+    apply vec_map_fun_ext.
+    intros.
+    etransitivity.
+    { apply ZE_mixed_subst_ren. }
+    apply ZE_mixed_subst_ext.
+    intro n.
+    (* ca devrait marcher *)
+  unfold shiftₙ, shiftₙₛ.
+  cbn -[leb].
+  cbn -[leb].
+  destruct (n <? a) eqn:eqna.
+  + rewrite ZE_ren_var;rewrite eqna; reflexivity.
+  + cbn -[leb].
+    rewrite 2 ZE_ren_ren.
+    rewrite 2 ZE_ren_subst_eq.
+    apply ZE_subst_ext.
+    intro.
+    unfold compose.
+    cbn -[leb].
+    f_equal.
+    case(Nat.ltb_spec _ _).
+    * intro. exfalso. lia.
+    * intros. f_equal.
+      rewrite Nat.add_sub.
+      reflexivity.
+Qed.
+Lemma ZE_subst_ren
+  {E} (g : nat -> nat) (f : nat -> ZE E) (z : ZE E) :
+  ZE_ren g (z [f ]ₘ) = z [fun n : nat => ZE_ren g (f n) ]ₘ.
+Proof.
+  revert z.
+  apply class_ind.
+  intro z.
+  fold (projE z).
+  rewrite ZE_subst_proj.
+  rewrite ZE_subst_proj.
+  apply ZE_mixed_subst_ren.
+  Qed.
+
+Fixpoint ZE_mixed_subst_subst {E : equational_theory}
+      (f g : nat -> ZE E) (z : Z _) :
+  (z ⟦ g ⟧) [f ]ₘ = z ⟦ fun n : nat => g n [f ]ₘ ⟧.
+Proof.
+  destruct z.
+  - reflexivity.
+  - cbn.
+    rewrite ZE_ops_subst.
+    f_equal.
+    rewrite vec_map_map.
+    apply vec_map_fun_ext.
+    intros a z.
+    etransitivity.
+    {apply ZE_mixed_subst_subst.}
+    apply ZE_mixed_subst_ext.
+    intro n.
+  unfold shiftₛ, shiftₙₛ.
+  case  (Nat.ltb_spec _ _) .
+    + rewrite ZE_subst_var.
+      case  (Nat.ltb_spec _ _).
+      reflexivity.
+      lia.
+  + cbn -[leb].
+    intros.
+    rewrite ZE_ren_subst.
+    rewrite ZE_subst_ren.
+    apply ZE_subst_ext.
+    intro.
+
+    case(Nat.ltb_spec _ _).
+    * intro. exfalso. lia.
+    * intros. f_equal.
+      rewrite Nat.add_sub.
+      symmetry.
+      apply ZE_ren_subst_eq.
+Qed.
+    (* ah mais c'est comme avant.. *)
+Lemma ZE_subst_subst {E : equational_theory}
+      (f g : nat -> ZE E) (x : ZE E) :
+  (x [g]ₘ) [f]ₘ = x [fun n : nat => g n [f]ₘ]ₘ.
+Proof.
+  revert x.
+  apply class_ind.
+  intro z.
+  fold (projE (E := E) z).
+  rewrite ZE_subst_proj.
+  rewrite ZE_subst_proj.
+  apply ZE_mixed_subst_subst.
+Qed.
+Fixpoint ZE_mixed_subst_id {E}(z : Z _): z ⟦ VarE ⟧ = z / ZEr E.
+Proof.
+  destruct z.
+  - reflexivity.
+  - cbn.
+    etransitivity;revgoals.
+    apply ZE_ops_projE.
+    f_equal.
+    apply vec_map_fun_ext.
+    intros n z.
+    etransitivity;[|apply ZE_mixed_subst_id].
+    apply ZE_mixed_subst_ext.
+    intro m.
+    apply shiftₙₛ_var.
+    apply ZE_ren_var.
+Qed.
+
+Lemma ZE_subst_id {E} (z : ZE E) : z [VarE ]ₘ = z.
+Proof.
+  revert z.
+  apply class_ind.
+  intro z.
+  etransitivity.
+  apply ZE_subst_proj.
+  apply ZE_mixed_subst_id.
+Qed.
 Program Definition ZEModel ( E : equational_theory) : model (main_signature E) :=
-  {| data := ZEModel_data E |}.
-Next Obligation.
-Admitted.
+  {| data := ZEModel_data E ;
+     laws := {|
+              substitution_ext := @ZE_subst_ext E ;
+              variables_subst := @ZE_subst_var E ;
+              ops_subst := @ZE_ops_subst E ;
+              assoc := @ZE_subst_subst E ;
+              id_neutral := @ZE_subst_id E
+            |}
+  |}.
+
+Definition projE_mor {E} : model_mor (ZModel _) (ZEModel E) :=
+  {| carrier_mor := (projE : ZModel _ -> ZEModel E) ;
+     substitution_mor := fun f z => eq_sym (ZE_subst_proj_proj f z) ;
+     variables_mor := fun _ => eq_refl _  ;
+     ops_mor := fun o v => eq_sym (ZE_ops_projE v)
+  |}.
+
 
 Fixpoint ini_mor_compat {E} (m : model_equational E)( x y : Z (main_signature E))(r :  ZEr E x y) :
   ini_mor m x = ini_mor m y.
@@ -818,7 +1436,6 @@ f z = ini_morE m z.
   rewrite ini_morE_proj.
   Abort.
 (*
-  destruct (lift_fun f : ) as [h feq].
   apply factor_extens.
   revert z.
   unshelve eapply factor.
